src/SynthesisFacts.v
@@ -1,0 +1,113 @@
+Require Import Bool List String Peano_dec.
+Require Import Common FMap Syntax Semantics SemFacts StepDet StepSeq.
+Require Import Serial SerialFacts Simulation Predicate Synthesis.
+
+Lemma addPMsg_nil:
+  forall pmsg,
+    addPMsg pmsg nil = nil.
+Proof.
+  reflexivity.
+Qed.
+
+Lemma addPMsgs_nil:
+  forall pmsgs,
+    addPMsgs pmsgs nil = nil.
+Proof.
+  induction pmsgs; simpl; intros; auto.
+Qed.
+
+Lemma addPMsg_init:
+  forall pmsg objs,
+    getObjectStatesInit (addPMsg pmsg objs) =
+    getObjectStatesInit objs.
+Proof.
+  induction objs; simpl; intros; [reflexivity|].
+  find_if_inside; simpl; auto.
+  rewrite IHobjs.
+  reflexivity.
+Qed.
+
+Lemma addPMsgs_init:
+  forall pmsgs objs,
+    getObjectStatesInit (addPMsgs pmsgs objs) =
+    getObjectStatesInit objs.
+Proof.
+  induction pmsgs; simpl; intros; [reflexivity|].
+  rewrite IHpmsgs.
+  apply addPMsg_init.
+Qed.
+
+Lemma addPMsgsSys_init:
+  forall pmsgs sys,
+    getStateInit (addPMsgsSys pmsgs sys) = getStateInit sys.
+Proof.
+  unfold addPMsgsSys; simpl; intros.
+  unfold getTStateInit; simpl.
+  rewrite addPMsgs_init.
+  reflexivity.
+Qed.
+
+Lemma addPMsg_indices:
+  forall pmsg objs,
+    map (fun o => obj_idx o) (addPMsg pmsg objs) =
+    map (fun o => obj_idx o) objs.
+Proof.
+  induction objs; simpl; intros; [reflexivity|].
+  find_if_inside; simpl; auto.
+  rewrite IHobjs; reflexivity.
+Qed.
+
+Lemma addPMsgs_indices:
+  forall pmsgs objs,
+    map (fun o => obj_idx o) (addPMsgs pmsgs objs) =
+    map (fun o => obj_idx o) objs.
+Proof.
+  induction pmsgs; simpl; intros; [reflexivity|].
+  rewrite IHpmsgs.
+  apply addPMsg_indices.
+Qed.
+
+Lemma addPMsgsSys_indices:
+  forall pmsgs sys,
+    indicesOf (addPMsgsSys pmsgs sys) = indicesOf sys.
+Proof.
+  unfold addPMsgsSys; simpl; intros.
+  unfold indicesOf; simpl.
+  apply addPMsgs_indices.
+Qed.
+
+Theorem simulation_pmsgs_compositional:
+  forall {StateS LabelS: Type} `{HasInit StateS} `{HasLabel LabelS}
+         (stepS: Step StateS LabelS)
+         impl1 impl2 spec simR simP
+         (Hii: iisOf impl1 = iisOf impl2)
+         (Hsim1: Simulates step_det stepS simR simP impl1 spec)
+         (Hsim2: Simulates step_det stepS simR simP impl2 spec)
+         impl (Himplii: iisOf impl = iisOf impl1)
+         (Himplp: SubList (pmsgsOf impl) (pmsgsOf impl1 ++ pmsgsOf impl2)),
+    Simulates step_det stepS simR simP impl spec.
+Proof.
+  unfold Simulates; intros.
+  specialize (Hsim1 ist1 sst1 H1 ilbl ist2).
+  specialize (Hsim2 ist1 sst1 H1 ilbl ist2).
+
+  destruct ilbl.
+  - apply Hsim1.
+    eapply step_det_in_pmsgs_weakening; eauto.
+    apply iisOf_indicesOf; auto.
+  - destruct mhdl as [hdl|];
+      [|inv H2; apply Hsim1; constructor].
+
+    pose proof (step_det_pmsgs_in _ _ _ _ H2) as Hhdl.
+    simpl in Hhdl; destruct Hhdl as [hpmsg [? ?]].
+    specialize (Himplp _ H3).
+    apply in_app_or in Himplp.
+    destruct Himplp.
+
+    + apply Hsim1.
+      admit.
+    + apply Hsim2.
+      admit.
+    
+Admitted.
+
